一个挺有意思的递推。

设 $f_{i,j}=\sum_{k=j}^n{a_k==a_i}$，则有以下转移：

$f_{i,j}=f_{i,j+1}+(a_j==a_i)$。

另设 $g_{i,j}=\sum_{k=i+1}^{j-1}{f_{k,j}}$，则有 $ans=\sum_{i=1}^n\sum_{j=i+1}^n{c_{i,j}}$，其中 $c_{i,j}$ 表示 $a_i=a_j$ 时的 $f_{i,j}$。

```cpp
#include <bits/stdc++.h>- 
using namespace std;
int t,n,a[3005];
long long f[3005][3005],g[3005][3005];
int main(){
    scanf("%d",&t);
    while(t--){
        long long ans=0;
        scanf("%d",&n);memset(f,0,sizeof(f));memset(g,0,sizeof(g));
        for(int i=1;i<=n;i++)scanf("%d",&a[i]);
        for(int i=1;i<=n;i++)
        for(int j=n;j>=1;j--)f[i][j]=f[i][j+1]+(a[j]==a[i]);//倒序递推f
        for(int j=1;j<=n;j++)
        for(int i=j-2,k=0;i>=1;i--)g[i][j]=(k+=f[i+1][j+1]);//倒序递推g
        for(int i=1;i<=n;i++)
        for(int j=i+1;j<=n;j++)if(a[i]==a[j])ans+=g[i][j];//统计答案
        printf("%lld\n",ans);
    }
    return 0;
}
```