令 $S_n=\sum_{i=1}^n c_i$

通过找规律可得（不必作过多阐述）：

$ans_{i,T}=\frac{S_n \times (n-2)((n-1)^T-1)}{(n-1)^2-1}+c_i=\frac{S_n \times (n-2)((n-1)^T-1)}{n^2-2n}+c_i=\frac{S_n \times ((n-1)^T-1)}{n}+c_i$

注意逆元。

由费马小定理可得 $a^{-1} \equiv a^{p-2} (\ mod \ p)$，由此可以解决有关 $\frac{1}{n}$ 的取余问题。

## AC Code:
```cpp
#include<bits/stdc++.h>
using namespace std;
typedef long long ll;
const int N=5e4+1;
ll n,T,t,a[N],sum,ans[N],mod=98765431;
ll power(ll x,ll y)
{
	ll ans=1;
	for(;y;y>>=1){
		if(y&1) ans=(ans*x)%mod;
		x=(x*x)%mod;
	}
	return ans;
}
int main()
{
	scanf("%lld%lld",&n,&T);
	for(int i=1;i<=n;i++){
		scanf("%lld",&a[i]);
		a[i]%=mod;
		sum=(sum+a[i])%mod;
	} 
	if(T%2==1) t=T-1;
	else t=T;
	for(int i=1;i<=n;i++){
		ans[i]=(power(n-1,t)-1)%mod*sum%mod+(a[i]*n%mod)%mod;
		ans[i]=(ans[i]*power(n%mod,mod-2))%mod;
	}
	sum=0;
	for(int i=1;i<=n;i++) sum=(sum+ans[i])%mod;
	if(T%2==1) for(int i=1;i<=n;i++) ans[i]=((sum-ans[i])+mod)%mod;
	for(int i=1;i<=n;i++) printf("%lld\n",ans[i]);
	return 0;
}
```