令 $g_i$ 为容斥系数。

使得 $\sum_{i}^{t} \binom{t}{i} g_i = [2 \nmid t]$。

令 $f_t = [2\nmid t]$。

二项式反演 $f_t = \sum_{i}^{t} \binom{t}{i} g_i \iff g_t = \sum_{i}^{t} (-1)^{t-i} \binom{t}{i}f_i$。


然后我们发现 $f_i$ 在 $[2 \mid i]$ 的时候没有贡献。

$g_t = (-1)^{t-1} \sum_{i}^{t}\binom{t}{i}f_i$。

考虑后面半部分 $\sum_{i}^{t} \binom{t}{i}1^{t-i}f_i$。

二项式定理$(x+y)^n = \sum_{k}^{n}\binom{n}{k}x^{n-k}y^k$。

考虑 $f_i$ 是交替的 0/1。整体乘上 $2$ 就可以认为 $f'_i = 1$。

$(1+1)^n = \sum_{k}^{n}\binom{n}{k} 1^{n-k}1^k$。

那么 $\sum_{k}^{n}\binom{n}{k} 1^{n-k}1^k = \sum_{i}^{t} \binom{t}{i}1^{t-i}f_i \times 2$

所以 $g_t = (-1)^{t-1} \times \frac{(1+1)^t}{2} = (-2)^{t-1}$

然后暴力状压就做完了。