高精度+gcd(f(m),f(n))=f(gcd(m,n))


证:gcd(f(m),f(n))=f(gcd(m,n))

引理1：

Gcd(F[n+1],F[n])=1;

证明：

根据辗转相减法则


```cpp
Gcd(F[n+1],F[n])
=Gcd(F[n+1]-F[n],F[n])
=Gcd(F[n],F[n-1])
=Gcd(F[2],F[1])
=1
```
引理2：


F[m+n]=F[m-1]F[n]+F[m]F[n+1]

证明：


F[n+m]
=F[n+m-1]+F[n+m-2]

=2\*F[n+m-2]+F[n+m-3]

=……


设
F[n+m]

=a[x]\*F[n+m-x]+b[x]\*F[n+m-x-1];

=a[x]\*(F[n+m-x-1]+F[n+m-x-2])+b[x]\*(F[n+m-x-1);

=(a[x]+b[x])\*F[n+m+x-1]+a[x]\*F[n+m+x-2];

当x=1时有 a[1]=F[2]; b[1]=F[1];

当x=2时有 a[2]=F[2]+F[1]=F[3]; b[2]=a[1]=F[2];

当x=k+1时有 a[k+1]=a[k]+b[k]=F[k+1]+F[k]=F[k+2] b[k+1]=a[k]=F[k+1];


所以当x=n时有



F[n+m]=a[n]F[m]+b[n]F[m-1];

=F[n+1]F[m]+F[n]F[m-1];

引理3：



Gcd(F[n+m],F[n])=Gcd(F[n],F[m])

证明：


```cpp
Gcd(F[n+m],F[n])
=Gcd(F[n+1]F[m]+F[n]F[m-1],F[n]);
=Gcd(F[n+1]F[m],F[n]);
=Gcd(F[n+1],F[n])*Gcd(F[m],F[n])
=Gcd(F[m],F[n]);
```
于是显然有：Gcd(F[n],F[m])=F[Gcd(n,m)];

```cpp
#include<cstdio>
    int x,y,k;
    struct node{int a[10001]={0};int l=1;} f[4];
    int n;
int gcd(int x,int y)
{
    return y!=0?gcd(y,x%y):x;
}
void jia(node x,node y,node &z)
{
    z.l=y.l;
    for(int i=1;i<=z.l;i++)
        z.a[i]=0;
    for(int i=1;i<=y.l;i++)
    {
        z.a[i]=z.a[i]+x.a[i]+y.a[i];
        z.a[i+1]=z.a[i+1]+z.a[i]/10;
        z.a[i]=z.a[i]%10;
    }
    z.l++;
    while(z.a[z.l]==0&&z.l>1)
        z.l--;
}
int main()
{
    scanf("%d %d",&x,&y);
    n=gcd(x,y);
    if(n==1)
    {
        printf("1");
        return 0;
    }
    if(n==2)
    {
        printf("1");
        return 0;
    }
    f[1].a[1]=1;
    f[2].a[1]=1;
    for(int i=3;i<=n;i++)
    {
        jia(f[1],f[2],f[3]);
        f[1]=f[2];
        f[2]=f[3];
    }
    if(f[3].l<=8)
    {
        for(int i=f[3].l;i>=1;i--)
            printf("%d",f[3].a[i]);
    }
    else
    {
        for(int i=8;i>=1;i--)
            printf("%d",f[3].a[i]);
    }
}
```