$\ \ \ \ \sum_{i=1}^{n}\sum_{j=1}^{m}(i \times j \operatorname{mod} p)$

$=\sum_{i=1}^{n}\sum_{j=1}^{m}( (i \operatorname{mod} p) \times (j \operatorname{mod} p)\operatorname{mod} p)$

考虑枚举 $(i \operatorname{mod} p)$ 和 $(j \operatorname{mod} p)$ 。

令 $f(n,k)=\sum_{i=1}^{n} [(i \operatorname{mod} p)=k]$

则式子可以表示为： $\sum_{k_1=0}^{p-1}\sum_{k_2=0}^{p-1} (i \times j \operatorname{mod} p) \times f(n,k_1) \times f(m,k_2)$

而简单推式子可得 $f(n,k)=\lfloor \frac{n+k}{p} \rfloor$

那么代码也很简单了

```cpp
R(n,m,p);
fo(i,0,p-1) a[i]=(n+i)/p;
fo(i,0,p-1) b[i]=(m+i)/p;
fo(i,1,p-1) fo(j,1,p-1) ans+=(i*j%p)*a[i]%mod*b[j]%mod;
write(ans%mod);
```

`R` 和 `write` 分别是快读快输。

`fo(i,a,b)` 表示循环变量为 `i` ，从 `a` 循环到 `b` 。