#### 我们先对这个式子进行化简：
 
 $ (1+2+...+N)×10000×1/N $

$ =n(n+1)/2 ×10000×1/N$

$ =n(n+1)×5000×1/n$

$ =5000×(n+1) $

```
Q:（1+2+...+N)×10000×1/N  为啥可以化简为 n(n+1)/2 ×10000×1/N  ?
```


```
A:想想高斯是如何做  1+2+3+...+99+100的。
   1+2+3+...+99+100
  =(1+100)+(2+99)+(3+98)+...+(50+51)
  =(1+100)*100/2
  =101*50
  =5050
  
  同理：
   1+2+3+4+...+n
  =(1+n)+(2+n-1）+（3+n-2）+(4+n-3)+...
  =(1+n)*n/2
  
  因此，
   （1+2+...+N)×10000×1/N 
   =(1+n)*n/2×10000×1/N 
```

因此，我们只要输出5000(n+1)的值就可以了！

代码如下：

```
#include<iostream>
#include<string>
using namespace std;
int main(){
	long long n;
	cin>>n;
	cout<<5000*(n+1)<<endl;
	return 0;
}
```
