下证$i+j=2^p$时,$f(i,j)=p-1$;

只须证明$f(i,j)=f(2^{p-1},2^{p-1})+p-1=p-1$

考虑采用数学归纳法。

显然对任意$m$满足$1<=m<=p-1$,若$f(i,j)=f(x,y)+m$,则$x+y=i+j$。

待证命题:对于任意$m$满足$1<=m<=p-1$,$f(i,j)=f(x,y)+m$,都有$2^m||x$,$2^m||y$(则当$m=p-1$时,有$f(i,j)=f(x0,y0)+p-1$,则必有$2^{p-1}||x0$,$2^{p-1}||y0$,又$x0+y0=i+j=2^p$,所以$x0=y0=2^{p-1}$,即可证明原命题)。
当$m=1$时,显然有$2||i-j$,$2||2j$;
设当$m=k$时结论成立,则$f(i,j)=f(ai+bj,ci+dj)+k$,由归纳假设$2^k||(ai+bj)$,$2^k||(ci+dj)$;
($a,b,c,d$为常数)

由对称性不妨设$ai+bj>ci+dj$;

则只需证$m=k+1$时,$f(i,j)=f((a-c)i+(b-d)j,2bi+2dj)+k-1$中的$(a-c)i+(b-d)j$,$2bi+2dj$均恰被整除即可。

注意到$2^{k+1}||2bi+2dj$,则只需证$2^{k+1}||(a-c)i+(b-d)j$即可。
不妨设$ai+bj=e*2^k$(此$e$非彼$e$),$ci+dj=f*2^k$;

(由条件可知$e,f$均为奇数且满足$2||e-f$,因为$e+f=2^{p-k}$,则有$e\equiv{-f(mod2^{p-k})}$,${(e-f)/2}\equiv{e(mod2^{p-k+1})}$,则有$2||(e-f)$ )
则$2^(k+1)=2*2^k||(e-f)*2^k=(a-c)i+(b-d)j$,即$2^{k+1}||(a-c)i+(b-d)j$
