由于 $b_i = a_i \operatorname{xor} a_{i + 1}$，那么 $b_{i - 1} = a_{i - 1} \operatorname{xor} a_i$。

那么可以得出这样一个结论：$a_i = b_{i - 1} \operatorname{xor} a_{i - 1}$。

原因也是很简单的。

$$
\begin{aligned}
b_{i - 1} &= a_i \operatorname{xor} a_{i - 1} \\
b_{i - 1} \operatorname{xor} a_{i - 1} &= a_i \operatorname{xor} a_{i - 1} \operatorname{xor} a_{i - 1}
\end{aligned}
$$

通过归零律（$a \operatorname{xor} a = 0$）得出：

$$
\begin{aligned}
b_{i - 1} \operatorname{xor} a_{i - 1} &= a_i \operatorname{xor} 0
\end{aligned}
$$

通过恒等律（$a \operatorname{xor} 0 = a$）得出：
$$
\begin{aligned}
b_{i - 1} \operatorname{xor} a_{i - 1} &= a_i \\
a_i &= b_{i - 1} \operatorname{xor} a_{i - 1}
\end{aligned}
$$

所以结论正确，而 $a_1$ 为 $0$ 即可，最后再判断一下，是否是无解，无解输出`-1`。

Code：
```cpp
#include <iostream>
#include <cstdio>
using namespace std;
int a[100001], b[100001];
int main() {
    int l;
    cin >> l;
    for (int i = 1; i <= l; ++i) cin >> b[i];
    a[1] = 0;
    for (int i = 2; i <= l; ++i) a[i] = (b[i - 1] ^ a[i - 1]);
    for (int i = 1; i < l; ++i)
        if ((a[i] ^ a[i + 1]) != b[i])
            return puts("-1"), 0;
    if ((a[l] ^ a[1]) != b[l]) return puts("-1"), 0;
    for (int i = 1; i <= l; ++i) cout << a[i] << endl;
}
```