
已知：

$A_i=B_{i-1}+C_{i-1}$ ，

$B_i=C_{i-1}+A_{i-1}$ ，

$C_i=A_{i-1}+B_{i-1}$ ，

求 $A_k-B_k$ 。

三种方法 。

### 法1

$A_k-B_k=(B_{k-1}+C_{k-1})-(C_{k-1}+A_{k-1})$

 $ \ \ \ \ \ \ \ \ \ \ \ \ \ \ \ \ =B_{k-1}-A_{k-1}$
 
 $ \ \ \ \ \ \ \ \ \ \ \ \ \ \ \ \ =(-1)^k(A_{0}-B_{0})$
 
 ```cpp
#include <iostream>

using namespace std;

int a,b,c,k;


int main() 
{
    int i,j,k;
    cin>>a>>b>>c>>k;
    cout<<(-(k%2*2-1))*(a-b);
	return 0;
}

```

### 法2
 
令$S_k=A_k+B_k+C_k=2(A_{k-1}+B_{k-1}+C_{k-1})=2^k(A_0+B_0+C_0)$ 
 
$A_k=B_{k-1}+C_{k-1}$

$ \ \ \ \ \ \ =A_{k-2}+S_{k-2}$

$ \ \ \ \ \ \ =A_{k-2}+2^{k-2}(A_0+B_0+C_0)$

若$2|k$

$A_k=\sum_{i=1}^{\frac{k}{2}-1}4^i(A_0+B_0+C_0)+A_0$

$B_k=\sum_{i=1}^{\frac{k}{2}-1}4^i(A_0+B_0+C_0)+B_0$

$C_k=\sum_{i=1}^{\frac{k}{2}-1}4^i(A_0+B_0+C_0)+C_0$

若$2|k+1$

$A_k=2\sum_{i=1}^{\frac{k}{2}-1.5}4^i(A_0+B_0+C_0)+B_0+C_0$

$B_k=2\sum_{i=1}^{\frac{k}{2}-1.5}4^i(A_0+B_0+C_0)+A_0+C_0$

$C_k=2\sum_{i=1}^{\frac{k}{2}-1.5}4^i(A_0+B_0+C_0)+A_0+B_0$

此时若是还没有发现 $A_k-B_k$ 能够消掉那么可以用一些等比数列求和公式加快速幂。

### 法3

考虑暴力方法。

$\begin{pmatrix}
A_i\\B_i\\C_i 
\end{pmatrix}\begin{pmatrix}
0&1&1\\1&0&1\\1&1&0 
\end{pmatrix}=\begin{pmatrix}
A_{i+1}\\B_{i+1}\\C_{i+1} 
\end{pmatrix}$

所以

$\begin{pmatrix}
A_{k}\\B_{k}\\C_{k} 
\end{pmatrix}=\begin{pmatrix}
A_0\\B_0\\C_0 
\end{pmatrix}\begin{pmatrix}
0&1&1\\1&0&1\\1&1&0 
\end{pmatrix}^k$

用矩阵快速幂求之 。