## 简要分析

先推一波式子

$$
\begin{aligned}

A_i-B_i&=(B_{i-1}+C_{i-1})-(A_{i-1}+C_{i-1}) \\

&=B_{i-1}-A_{i-1} \\

&=(-1) \times (A_{i-1}-B_{i-1})

\end{aligned}
$$

所以我们可以得到下面这个式子

$$
A_k-B_k=(-1)^k \times (A_0-B_0)
$$

因为 $1 \leq A_0,B_0,C_0 \leq 10^9$，即 $|A_0-B_0| \leq 10^{18}$，所以根本不需要判断 "Unfair" 的情况

## 完整代码

```cpp
#include <bits/stdc++.h>
#define int long long
#define ri register int
using namespace std;
int a, b, c, k;
template <typename T>
inline void read(T &x)
{
	register T f = 0, c = getchar();
	for (; c < 48 || 57 < c; c = getchar())
		if (c == '-')
			f = 1;
	for (x = 0; 48 <= c && c <= 57; c = getchar())
		x = (x << 3) + (x << 1) + (c & 15);
	if (f)
		x = ~(--x);
}
template <typename T>
inline void print(T x)
{
	if (x < 0)
		putchar('-'), x = ~(--x);
	if (x > 9)
		print(x / 10);
	putchar(x % 10 | 48);
}
signed main()
{
	read(a), read(b), read(c), read(k), print((k & 1 ? -1 : 1) * (a - b));
	return 0;
}
```
