设$x$为吃糖果的次数，则可列出方程：$(n-x+1)(n-x)=2(k+x)$。

化简可得：$x^2 -(2n+3)x+n^2+n-2k=0$

这个一元二次方程有可能出现$2$种解的情况，对于比$n$大的舍去即可。

代码：

```cpp
#include <bits/stdc++.h>
typedef long long ll;
using namespace std;
ll n, k, a, b, c, ans, qaq;
int main() {
	cin >> n >> k;
	a = 1;
	b = -((n << 1) + 3);
	c = (ll)n * n + n - (k << 1);
	ans = ((-b + (ll)sqrt((ll)(b * b) - (ll)(4 * a * c))) / (a << 1)) > n ? ((-b - (ll)sqrt((ll)(b * b) - (ll)(4 * a * c))) / (a << 1)) :((-b + (ll)sqrt((ll)(b * b) - (ll)(4 * a * c))) / (a << 1));
	cout << ans << endl;
	return 0;
}
```
