设添加x次   
则 最终结果为 $\frac{x(x+1)}2-(n-x)=k $    
移项得$x(x+3)=2(n+k)$    
因为$x(x+3)$在正数域上单调，二分即可    

```cpp
#include<iostream>
#include<cstdio>
#include<cstring>
#include<queue>
#define ll long long
#define inf 0x3f3f3f3f
using namespace std;
ll n,k;
inline ll read(){
	ll x=0,f=1;char ch=getchar();while(ch<'0'||ch>'9'){if(ch=='-')f=-f;ch=getchar();
	}while(ch>='0'&&ch<='9'){x=(x<<3)+(x<<1)+ch-'0';ch=getchar();
	}return x*f;
}
int main()
{
	n=read();k=read();
	ll l=0,r=n;
	while(l<r){
		ll mid=(l+r)>>1;
		if((ll)((mid*mid+3*mid)/2)<n+k)l=mid+1;else r=mid;
	} 
	printf("%lld\n",n-l);
	return 0;
}
```
