思路孔爷讲的很清楚了。

我来补一发fhq treap的代码。

```
//by zykykyk
#include<cstdio>
#include<ctime>
#include<cmath>
#include<cstring>
#include<algorithm>
#include<string>
#include<set>
#include<vector>
#include<queue>
#include<map>
#define rg register
#define il inline
#define vd void
#define ll long long
#define N 100010
#define For(i,x,y) for (int i=(x);i<=(y);i++)
#define Dow(i,x,y) for (int i=(x);i>=(y);i--)
#define cross(i,k) for (int i=first[k];i;i=last[i])
using namespace std;
il int read(){
    int x=0;int ch=getchar(),f=1;
    while (!isdigit(ch)&&(ch!='-')&&(ch!=EOF)) ch=getchar();
    if (ch=='-'){f=-1;ch=getchar();}
    while (isdigit(ch)){x=(x<<1)+(x<<3)+ch-'0';ch=getchar();}
    return x*f;
}
il vd print(ll x){
    if (x<0) putchar('-'),x=-x;
    if (x>=10) print(x/10),putchar(x%10+'0');
        else putchar(x+'0');
}
int n,m,x,y,z,mid,ans_l,ans_r,ans_mid,a[N];
ll ans;

int root,tot,pri[N],size[N],son[N][2];
ll sum[N],val[N];
il int make_node(int v){
	size[++tot]=1;
	pri[tot]=rand();
	sum[tot]=val[tot]=v;
	return tot;
}
il vd pushup(int u){
	size[u]=size[son[u][0]]+size[son[u][1]]+1;
	sum[u]=sum[son[u][0]]+sum[son[u][1]]+val[u];
}
il vd Split(int u,int v,int &x,int &y){
	if (!u) x=y=0;
	else {
		if (val[u]<=v) x=u,Split(son[u][1],v,son[u][1],y);
		else y=u,Split(son[u][0],v,x,son[u][0]);
		pushup(u);
	}
}
il int Merge(int x,int y){
	if (!x||!y) return x+y;
	if (pri[x]<pri[y]){
		son[x][1]=Merge(son[x][1],y);
		pushup(x);
		return x;
	}
	else {
		son[y][0]=Merge(x,son[y][0]);
		pushup(y);
		return y;
	}
}
il int Kth(int u,int k){
	while (2333){
		if (size[son[u][0]]+1<k) k-=size[son[u][0]]+1,u=son[u][1];
		else if (size[son[u][0]]>=k) u=son[u][0];
		else return u;
	}
}
il vd insert(int v){
	Split(root,v,x,y);
	root=Merge(Merge(x,make_node(v)),y);
}
il vd Delete(int v){
	Split(root,v,x,z),Split(x,v-1,x,y);
	y=Merge(son[y][0],son[y][1]);
	root=Merge(Merge(x,y),z);
}
int main(){
	srand(time(0));
	n=read(),m=read();
	For(i,1,n) a[i]=read();
	ans=2333333333333333;
	For(i,1,n){
		insert(a[i]);
		if (i<m) continue;
		if (i!=m) Delete(a[i-m]);
		mid=val[Kth(root,(m>>1)+1)];
		Split(root,mid,x,z),Split(x,mid-1,x,y);
		ll Sum=1ll*mid*size[x]-sum[x]+sum[z]-1ll*mid*size[z];
		if (Sum<ans){
			ans=Sum;
			ans_l=i-m+1,ans_r=i,ans_mid=mid;
		}
		root=Merge(Merge(x,y),z);
	}
	print(ans),putchar('\n');
	For(i,1,n)
		if (i>=ans_l&&i<=ans_r) print(ans_mid),putchar('\n');
		else print(a[i]),putchar('\n');
}
```