#### 算法分析

注意到
$\sum\limits_{i = l}^r {{a_i}}  = r - l + 1 \Leftrightarrow \sum\limits_{i = l}^r {{a_i}}  - \sum\limits_{i = l}^r 1  = \sum\limits_{i = l}^r {\left( {{a_i} - 1} \right)}  = 0$，于是只需对每个元素$-1$，然后原问题就转化成统计和为$0$的子数组的个数。

#### C++代码
```cpp
#include <iostream>
#include <vector>
#include <map>
#define int long long

using namespace std;

int n;
string s;

signed main() {
	int t;
	cin >> t;
	
	while (t--) {
		cin >> n >> s;
		vector<int> v(n);
		for (int i = 0; i < n; ++i) v[i] = s[i] - '0' - 1;
		
		map<int, int> mp;
		int sum = 0, ans = 0;
		for (int i = 0; i < n; ++i) {
			sum += v[i];
			if (sum == 0) ans++;
			ans += mp[sum];
			mp[sum]++;
		}
		
		cout << ans << '\n';
	}
	
	return 0;
}
```
