令 $f_k=\sum_{i=0}^\infty i^kq^i$，那么

$qf_k=\sum_{i=0}^\infty i^kq^{i+1}$

$(1-q)f_k=q\sum_{i=0}^\infty((i+1)^k-i^k)q^i$

$=q \sum_{i=0}^{\infty} \sum_{j=0}^{k-1}\binom{k}{j} i^j q^i$

$=q\sum_{j=0}^{k-1}\binom{k}{j}\sum_{i=0}^\infty i^jq^i$

$=q\sum_{j=0}^{k-1}\binom{k}{j}f_j$

$f_k=\frac{q}{1-q}\sum_{i=0}^{k-1}\binom{k}{i}f_i$

$\frac{f_k}{k!}=\frac{q}{1-q}\sum_{i=0}^{k-1}\frac{f_i}{i!}\frac{1}{(k-i)!}$

$\frac{1}{1-q}F(x)=\frac{q}{1-q}F(x)e^x+\frac{1}{1-q}$

$F(x)=qF(x)e^x+1$

$F(x)=\frac{1}{1-qe^x}$

直接多项式求逆即可，时间复杂度 $O(m\log m)$