# Description

[P1487 失落的成绩单](https://www.luogu.com.cn/problem/P1487)

对于一个满足：
$$A_{i}=\dfrac{A_{i-1}-A_{i+1}}{2} + d$$
的数列 $a$，给出首项 $A_{1}$，末项 $A_{n}$，以及常数项 $d$。请求出 $A_{m}$ 的值。

数据范围：$1\le n\le 60$，$0\le m\le n$，$|d|,|A_1|,|A_n|<10^4$。
 
# Analysis
由：
$$A_{i}=\dfrac{A_{i-1}-A_{i+1}}{2} + d$$
得：
$$2A_{i}=A_{i-1}-A_{i+1}+2d$$
移项后：
$$A_{i+1}=A_{i-1}-2A_{i}+2d$$ 
令 $i=i-1$，得：
$$A_{i}=A_{i-2}-2A_{i-1}+2d$$
因为：
$$A_{3}=A_{1}-2A_{2}+2d$$
$$A_{4}=A_{2}-2A_{3}+2d$$
得：
$$
\begin{aligned}
A_{4}&=A_{2}-2(A_{1}-2A_{2}+2d)+2d\\
A_{4}&=A_{2}-2A_{1}+4A_{2}-4d+2d\\
A_{4}&=-2A_{1}+5A_{2}-2d
\end{aligned}
$$
则可以根据上式递推得此式：
$$A_{n}=\color{red}x\color{black}A_{1}+\color{red}y\color{black}A_{2}+\color{red}z\color{black}d$$
中的 $\color{red}x\color{black},\color{red}y\color{black},\color{red}z$，并推出：
$$A_{2}=\dfrac{A_{n}-\color{red}x\color{black}A_{1}-\color{red}z\color{black}d}{\color{red}y}$$
# CODE
```cpp
#include<stdio.h>
struct test
{
    int x, y, z;
} score[61];
int main()
{
    double a[61], d;
    int n, m;
    scanf("%d %d", &n, &m);
    scanf("%lf %lf %lf", &d, &a[1], &a[n]);
    score[3].x = 1, score[3].y = -2, score[3].z = 2;
    score[4].x = -2, score[4].y = 5, score[4].z = -2;
    for(int i = 5; i <= n; i++)
    {
        score[i].x = score[i-2].x - 2 * score[i-1].x;
        score[i].y = score[i-2].y - 2 * score[i-1].y;
        score[i].z = score[i-2].z - 2 * score[i-1].z + 2;
    }
    a[2] = (a[n] - score[n].x * a[1] - score[n].z * d) / score[n].y;
    for(int i = 3; i <= m; i++)
    {
        a[i] = a[i-2] - 2 * a[i-1] + 2 * d;
    }
    printf("%.3f",a[m]);
    return 0;
}
```