显然把$x^3$改成$x^2$就是水dp

于是考虑拆分：

$$(x+1)^3-x^3=\sum_{i=1}^3 C_i^3x^i=3x^2+3x+1$$

于是分开维护$x^2$和$x$的期望为$x1$,$x2$

由于$E(x+y)=E(x)+E(y)$显然我们$x1/2_i$就是$x1/2_{i-1}+\text{多的期望}$

多的期望分别是：


$$(x+1)^2 - x^2=x^2+2x+1-x^2=2x+1=2x2_{i-1}+1$$

$$x+1-x =1$$

于是轻松得出递推式：

$$x1_i=p_i(x1_{i-1}+2x2_{i-1}+1)$$

$$x2_i=p_i(x2_{i-1}+1)$$

$$ans_i=ans_{i-1}+p_i(3x1_{i-1}+3x2_{i-1}+1)$$

然后递推就好了。。。~~所以又水过了一道紫题~~

```cpp
#include <bits/stdc++.h>

using namespace std;

int n;
double d, x = 0.0 , y = 0.0, f = 0.0;

int main() {
	scanf("%d", &n);
	while (n--) {
		scanf("%lf", &d);
		f += (3 * (x + y) + 1) * d; 
		y = (y + 2 * x + 1) * d;
		x = (x + 1) * d; 
	}
	printf("%.1lf", f);
	return 0;
}
```
