#### 思路

看着就很像用前缀和吧。

首先，看到数据范围， $ c $ 很小。

于是定义 $ f[i][j][k] $ 为前 $ j \times k $ 个星星的亮度为 $ i $ 时的个数

则 $ f[i][j][k] \gets  f[i][j][k] + f[i][j - 1][k] + f[i][j][k - 1] - f[i][j - 1][k - 1] $

#### 代码

```
#include <bits/stdc++.h>
using namespace std;
const int Maxn = 1e5 + 5;
int n , q , c , x[Maxn] , y[Maxn] , p[Maxn];
int f[15][105][105] , T , A , B , C , D , Ans , Sum;
int main() {
	cin >> n >> q >> c;
	for(int i = 1 ; i <= n ; i ++) {
		cin >> x[i] >> y[i] >> p[i];
		f[p[i]][x[i]][y[i]]++;
	}
	for(int i = 0 ; i <= c ; i ++) {
		for(int j = 1 ; j <= 100 ; j ++) {
			for(int k = 1 ; k <= 100 ; k ++) {
				f[i][j][k] += f[i][j - 1][k] + f[i][j][k - 1] - f[i][j - 1][k - 1];
			}
		}
	}
	while(q--) {
		cin >> T >> A >> B >> C >> D;
		Ans = 0;
		for(int i = 0 ; i <= c ; i ++) {
			Ans += (i + T) % (c + 1) * (f[i][C][D] - f[i][C][B - 1] - f[i][A - 1][D] + f[i][A - 1][B - 1]);
		}
		cout << Ans << endl;
	}
	return 0;
}