写个不太一样的做法~

设 $F(n, m) = \sum_{k=0}^n k^mx^k\binom nk$，于是答案就是 $\sum_i a_iF(n, i)$。

那么有：
$$
\begin{aligned}
F(n, m) &= \sum_{k=0}^n k^m x^k \binom nk\\
&= n\sum_{k=0}^n k^{m-1}x^k\binom {n-1}{k-1}
\end{aligned}
$$
然后：
$$
\begin{aligned}
F(n, m) &= \sum_{k=0}^n k^mx^k\binom nk\\
&= \sum_{k=0}^n k^mx^k\left(\binom {n-1}k + \binom{n-1}{k-1} \right)\\
&= F(n-1,m) + \frac 1n F(n, m + 1)
\end{aligned}
$$
也就是说：$F(n, m) = n(F(n, m - 1) - F(n - 1, m - 1))$。

边界为 $F(n, 0) = (x + 1)^n$。

代码见我的 [$\texttt{blog}$](https://www.cnblogs.com/cj-xxz/p/13198301.html)