设 $f(x)= \log_2 ( lowbit(j))$

$\left\{f(x)\right\}=\left\{0,1,0,2,0,1,0,3,0……\right\}$

设 $b(x)=x$ 的二进制表示中 $1$ 的个数

设 $g(x)= \sum_{i=1}^x f(i)$

则 $g(x)=\sum_{i\ge1}(k\le n$ 且 $f(k)\ge i$ 的 $k$ 的个数 $)$

![](https://cdn.luogu.com.cn/upload/image_hosting/a2wmmdwg.png?x-oss-process=image/resize,m_lfit,h_680,w_900)

$=\sum_{i\ge1}\lfloor\dfrac{x}{2^i}\rfloor$

$=x-b(x)$

![](https://cdn.luogu.com.cn/upload/image_hosting/xm4zrrrn.png?x-oss-process=image/resize,m_lfit,h_680,w_900)

设 $h(x)=\sum_{i=0}^{2^x-1} b(x)$

则 $h(x)=h(x-1)+(h(x-1)+2^{x-1})$

$=2h(x-1)+2^{x-1}$

$=2(2h(x-2)+2^{x-2})+2^{x-1}$

$=4h(x-2)+2\times2^{x-1}$

$=4(2h(x-3)+2^{x-3})+2\times2^{x-1}$

$=8h(x-3)+3\times2^{x-1}$

$=$ ……

$=2^xh(0)+x\times2^{x-1}$

$=x\times2^{x-1}$

$\sum_{i=1}^{2^n} \log_2 (\prod_{j=1}^i lowbit(j))$

$=\sum_{i=1}^{2^n} \sum_{j=1}^i\log_2 ( lowbit(j))$

$=\sum_{i=1}^{2^n} g(i)$

$=\left( \sum_{i=1}^{2^n}i \right)-\left( \sum_{i=1}^{2^n}b(i) \right)$

$=\dfrac{2^{n}(2^n+1)}{2}-n2^{n-1}-1$

$=2^{n-1}(2^n+1)-n2^{n-1}-1$

所以在取模时只要先算 $k=2^{n-1}$ 就可以了。

**【代码】**
```cpp
#include<iostream>
#include<cstdio>
#define int long long
using namespace std;
int mod=1e9+7;
int n; 
int mod1(int x,int y)//取模
{return (x%y+y)%y;}
int pow2mod(int x)//2^x%mod快速幂
{
	if(x==0) return 1;
	if(x%2==1) return 2*pow2mod(x-1)%mod;
	int temp=pow2mod(x/2);
	return temp*temp%mod;
}
signed main()
{
	cin>>n;
	int k=pow2mod(n-1);
	n%=mod;k%=mod;
	printf("%lld",mod1( (k*(2*k+1)%mod)-(n*k%mod)-1 ,mod));
	return 0;
}
```
