## 思路

转化一下 $\sum_{i=c_1}^{c_2}\sum_{j=r_1}^{r_2}\dbinom{i+j}{i}$。

推一推 $\sum_{i=c_1}^{c_2}(\sum_{j=r_1}^{r_2}\dbinom{i+j}{i}+\dbinom{i+r_1}{i+1}-\dbinom{i+r_1}{i+1})=\sum_{i=c_1}^{c_2}(\dbinom{i+r_2+1}{i+1}-\dbinom{i+r_1}{i+1})$。

再推一推 $\sum_{i=c_1}^{c_2}(\dbinom{i+r_2+1}{i+1}-\dbinom{i+r_1}{i+1})=\dbinom{c_2+r_2+2}{c_2+1}-\dbinom{c_1+r_2+1}{c_1}-\dbinom{c_2+r_1+1}{r_1}+\dbinom{r_1+c_1}{r_1}$。

然后就没有然后了。

不清楚这个式子的可以观察杨辉三角或自己把组合数拆开：

$\dbinom{i}{j}+\dbinom{i}{j+1}=\dfrac{i!}{j!(i-j)!}+\dfrac{i!}{(j+1)!(i-j-1)!}=\dfrac{((j+1)+(i-j))i!}{(j+1)!(i-j)!}=\dfrac{(i+1)!}{(j+1)!(i-j)!}=\dbinom{i+1}{j+1}$。

## 代码

```cpp
#include <bits/stdc++.h>
#define int long long
#define double long double
#define mid ((l+r)>>1)
using namespace std;
const int mod=1e9+7;
int qp(int a,int b){
	int ans=1;
	while(b){
		if(b&1) ans=(ans*a)%mod;
		a=(a*a)%mod;
		b>>=1;
	}
	return ans;
}
int fac[10000005],inv[10000005];
void init(){
	fac[0]=1;
	for(int i=1;i<=10000000;i++) fac[i]=fac[i-1]*i%mod;
	inv[10000000]=qp(fac[10000000],mod-2);
	for(int i=9999999;i>=0;i--) inv[i]=inv[i+1]*(i+1)%mod;
}
int C(int i,int j){
	if(i<0||j<0||i<j) return 0;
	return fac[i]*inv[i-j]%mod*inv[j]%mod;
}
signed main(){
	init();
	int r1,c1,r2,c2;
	cin>>r1>>c1>>r2>>c2;
	cout<<(C(r2+1+c2+1,r2+1)+C(r1+c1,r1)+mod+mod-C(r1+c2+1,r1)-C(r2+c1+1,c1))%mod;
	return 0;
}
```