感觉这道题用阶乘做挺巧妙的，所以说决定水一发：


设$f(i) = i!\ mod\ p$ , $g(i) = i!^{-1}\ mod\ p$


$g(i) = g(i+1) * (i+1) $


$i^{-1} = f(i-1) * g(i)$


算出$f_n$然后求出$f_n$的逆元$g_n$，递推即可。


顺便宣传一波[博客](http://blog.csdn.net/charlie\_jilei/article/details/77122700)


代码：

```cpp

#include<cstdio>
#include<iostream>
using namespace std;
int mi[3000010];
int n,p;
int anss[3000100],g;
int fast_pow(int a,int x)
{
    int ans=1;
    for (;x;x>>=1,a=(1ll*a*a)%p)
        if (x&1) ans=(1ll*ans*a)%p;
    return ans;
}
int main()
{
    scanf("%d%d",&n,&p);
    mi[0]=1; 
    for (int i=1;i<=n;i++)
        mi[i]=(1ll*mi[i-1]*i)%p;
    g=fast_pow(mi[n],p-2);
    anss[n]=(1ll*g*mi[n-1])%p;
    for (int i=n-1;i;i--)
    {
        g=(1ll*g*(i+1))%p;
        anss[i]=(1ll*g*mi[i-1])%p;
    }
    for (int i=1;i<=n;i++)
        printf("%d\n",anss[i]);
}
```