其实有一种非常好理解的线性做法

首先算出1!~n!

然后费马小算出n!的逆元，再由$ n!^{-1}=(n+1)!^{-1}*(n+1) $ 倒推 1!~(n-1)! 的逆元

最后由 $ x^{-1}=x!*(x-1)!^{-1} $ 求出1~n的逆元
```cpp
#include<bits/stdc++.h>
#define ll long long
#define For(i,j,k) for(register int i=j;i<=k;i++)
using namespace std;
int read(){
    int x=0,l=1; char ch=getchar();
    while(!isdigit(ch)) {if (ch=='-') l=-1; ch=getchar();}
    while(isdigit(ch)) x=x*10+(ch^48),ch=getchar();
    return x*l;
}
int l,buf[10],mo,n; ll c;
void write(int x){
    l=0;
    while(x) buf[++l]=x%10,x/=10;
    if(!l) l=1,buf[1]=0;
    while(l) putchar('0'+buf[l--]);
    putchar('\n');
}
int ksm(ll a,int b){
    c=1;
    while(b){
    	if (b&1) c=(c*a)%mo;
    	a=(a*a)%mo; b>>=1;
    }
    return c;
}
ll a[3000005],ny[3000005];
int main(){
    n=read(),mo=read(); a[1]=1;
    For(i,2,n) a[i]=a[i-1]*i%mo; ny[n]=ksm(a[n],mo-2);
    for(int i=n-1;i>=1;--i) ny[i]=ny[i+1]*(i+1)%mo; printf("1\n");
    For(i,2,n) write(a[i-1]*ny[i]%mo);
    return 0;
}
```