求
$$F(x)G(x)\equiv1\ ({\rm mod}\ x^n)$$
令
$$F(x)G_1(x)\equiv1\ ({\rm mod}\ x^{\left\lceil\frac{n}{2}\right\rceil})$$
作差可得
$$F(x)\big(G(x)-G_{1}(x)\big)\equiv0\ ({\rm mod}\ x^{\left\lceil\frac{n}{2}\right\rceil})$$
除去$F(x)$,得
$$G(x)-G_1(x)\equiv0\ ({\rm mod}\ x^{\left\lceil\frac{n}{2}\right\rceil})$$
两边平方，得
$$\big(G(x)-G_1(x)\big)^2\equiv0\ ({\rm mod}\ x^n)$$
展开有
$$G^2(x)-2G(x)G_1(x)+G^2_1(x)\equiv0\ ({\rm mod}\ x^n)$$
同时乘上$F(x)$，由定义，有
$$G(x)-2G_1(x)+F(x)G_1^2(x)\equiv0\ ({\rm mod}\ x^n)$$
求得递归式
$$G(x)\equiv2G_1(x)-F(x)G_1^2(x)\ ({\rm mod}\ x^n)$$
再提取一下公因式
$$G(x)\equiv G_1(x)\big(2-F(x)G_1(x)\big)\ ({\rm mod}\ x^n)$$
化简为常数项后直接求逆元即可
```cpp
#include <cstdio>
#include <iostream>
#define ll long long

using namespace std;
const int N = 3 * 1e+6 + 10, P = 998244353, G = 3, Gi = 332748118;
int n, m, lim = 1, L, rev[N];
ll a[N], b[N], c[N];

int read() {
	int x = 0, f = 1; char c = getchar();
	while(c < '0' || c > '9') {if(c == '-') f = -1; c = getchar();}
	while(c >= '0' && c <= '9') x = (x<<1) + (x<<3) + c - '0', c = getchar();
	return x * f;
}
ll qpow(ll a, ll b) {
	ll prod = 1;
	while(b) {
		if(b & 1) prod = prod * a % P;
		a = a * a % P;
		b >>= 1;
	}
	return (prod + P) % P;
}
void NTT(ll *A, int inv) {
	for(int i = 0; i < lim; i++)
		if(i < rev[i]) swap(A[i], A[rev[i]]);
	for(int mid = 1; mid < lim; mid <<= 1) {
		ll tmp = qpow(inv == 1 ? G : Gi, (P - 1) / (mid << 1));
		for(int j = 0; j < lim; j += (mid << 1)) {
			ll omega = 1;
			for(int k = 0; k < mid; k++, omega = (omega * tmp) % P) {
				int x = A[j + k], y = omega * A[j + k + mid] % P;
				A[j + k] = (x + y) % P;
				A[j + k + mid] = (x - y + P) % P;
			}
		}
	}
	if(inv == 1) return;
	int ny = qpow(lim, P - 2);
	for(int i = 0; i < lim; i++) A[i] = (1LL * A[i] * ny + P) % P;
}
void PI(ll *F, ll *G, int n) {
	if(n == 1) {
		G[0] = qpow(F[0], P - 2);
		return;
	}
	PI(F, G, (n + 1) >> 1);
	lim = 1, L = 0;
	while(lim < (n << 1)) lim <<= 1, L++;
	for(int i = 1; i < lim; i++) 
		rev[i] = (rev[i >> 1] >> 1) | ((i & 1) << (L - 1));
	for(int i = 0; i < n; i++) c[i] = F[i];
	for(int i = n; i < lim; i++) c[i] = 0;
	NTT(c, 1), NTT(G, 1);
	for(int i = 0; i < lim; i++) 
		G[i] = ((2LL - G[i] * c[i] % P) + P) % P * G[i] % P;
	NTT(G, -1);
	for(int i = n; i < lim; i++) G[i] = 0;
}
int main()
{
	n = read();
	for(int i = 0; i < n; i++) 
		a[i] = (read() + P) % P;
	PI(a, b, n);
	for(int i = 0; i < n; i++)
		printf("%d ", b[i]);
	return 0;
}
```
