令A=x-y;B=n-m;

可得到abs(A+B\*y)%l=0;

即A+B\*y=x\*l;

化简的B\*y-x\*l=-A;

这不就是就是拓展欧几里得吗；

上代码

```cpp
#include<iostream>
#include<cstdio>
#include<algorithm>
using namespace std;
typedef long long ll;
ll n,m,x,y,l,t;
ll b,a;
ll x1,y2,r,d;
int gcd(ll a,ll b,ll&x,ll&y)
{
    if(b==0)
    {
        x=1;y=0;
        return a;
    }
    d=gcd(b,a%b,x,y);
    int t=x;
    x=y;
    y=t-(a/b)*y;
    return d;
}
int main()
{
    scanf("%lld%lld%lld%lld%lld",&x1,&y2,&m,&n,&l);
     a=(x1-y2);
    b=(n-m);
    if(b<0)
    {
        a=-a;
        b=-b;
    }
    r=gcd(b,l,x,y);
    if(a%r!=0)
        printf("Impossible");
    else
    printf("%lld",((x*a/r)%(l/r)+(l/r))%(l/r));
return 0;
}
```