首先，

$$
\sum_{l = 1}^{n - 1}\sum_{r = l + 1}^{n}(a_l + a_r)^x = \frac{\sum\limits_{l = 1}^{n}\sum\limits_{r = 1}^{n}(a_l + a_r)^x - \sum\limits_{i = 1}^{n}(2a_i)^x}{2}
$$

然后对于 $\sum\limits_{i = 1}^{n}\sum\limits_{j = 1}^{n}(a_l + a_r)^x$，可以二项式定理展开。

$$
\begin{aligned}
\sum\limits_{l = 1}^{n}\sum\limits_{r = 1}^{n}(a_l + a_r)^x &= \sum_{l = 1}^{n}\sum_{r = 1}^{n}\sum_{i + j = x}\binom{x}{i}a_l^i a_r^j \\
&= \sum_{i + j = x}\binom{x}{i}\left(\sum_{l = 1}^{n}a_l^i\right)\left(\sum_{r = 1}^{n}a_r^j\right) \\
\end{aligned}
$$

暴力预处理 $b_x = \sum\limits_{i = 1}^{n}a_i^x$，即可快速算出所有答案。