根据插值公式有

$$
f(m+a)=\sum_{i=0}^nf(i)\prod_{j\neq i}\frac{m+a-j}{i-j}
$$

$$
=\sum_{i=0}^nf(i)\frac{(m+a)!\big((m+a-n-1)!(m+a-i)\big)^{-1}}{i!(n-i)!(-1)^{n-i}}
$$

$$
=\frac{(m+a)!}{(m+a-n-1)!}\sum_{k=0}^n\frac{f(k)}{k!(n-k)!(-1)^{n-k}}\frac{1}{m+a-k}
$$

无妨令 $\color{royalblue}{}^{[1]}$

$$
a_i=\frac{f(i)}{i!(n-i)!(-1)^{n-i}}\;\;(i\leqslant n),\quad b_i=\frac{1}{m-n+i}
$$

并令在 $i>n$ 时令 $a_i$ 为零，那么

$$
f(m+
a)=\left[z^{n+a}\right]\frac{(m+a)!A(z)B(z)}{(m+a-n-1)!}
$$

卷起来就完事了。

------------
$\small{\color{royalblue}{[1]}}:m$ 很大，不能直接设为 $b_i=\frac{1}{i}$，否则会一直 RE。