先令 $b_i = \lfloor a_i \rfloor$。

由于 $\sum a_i = 0$ 且 $\lfloor x \rfloor \leq x$，所以有 $\sum b_i \leq 0$。

可以发现将一个非整数 $a_i$ 从 $\lfloor a_i \rfloor$ 变成 $\lceil a_i\rceil$ 会使得总和增加 $1$。所以可以将 $0 - \sum b_i$ 个非整数 $a_i$ 从 $\lfloor a_i \rfloor$ 变成 $\lceil a_i\rceil$。

```cpp
#include <iostream>
#include <cstdio>
#include <algorithm>
#include <cmath>
#include <cstring>
using namespace std;

const int N = 1e5 + 5;

int n;
double a[N];
bool v[N];

int main()
{
	scanf("%d", &n);
	long long sum = 0;
	for (int i = 1; i <= n; i++)
	{
		scanf("%lf", &a[i]);
		v[i] = ((int)a[i]) == a[i];
		a[i] = floor(a[i]);
		sum += a[i];
	}
    long long need = 0 - sum;
	for (int i = 1; i <= n; i++)
	{
		if (v[i] || need == 0)
		{
			printf("%.0f\n", a[i]);
			continue;
		}
		printf("%.0f\n", a[i] + 1);
		need--;
	}
	return 0;
}
```
