**易错点：**
- 笔者由于没有进行数据初始化（排序以及数据填充）和状态转移中的一个字母r写成了l而调试了近一个小时.

------------
```cpp
#include<cstdio>
#include<iostream>
#include<algorithm>
#include<cstring>
#define ll long long
using namespace std;
const ll INF=0x3f3f3f3f3f3f3f3f;
const int MAXN=1e5+10,MAXP=110;
ll f[MAXP][MAXN],sumD[MAXN];
ll A[MAXN],sumA[MAXN];
int q[MAXN],l,r;
int main(){
	int n,m,p;
	scanf("%d%d%d",&n,&m,&p);
	for(int i=2;i<=n;i++){
		int d;
		scanf("%d",&d);
		sumD[i]=sumD[i-1]+d;
	}
	for(int i=1;i<=m;i++){
		int h,t;
		scanf("%d%d",&h,&t);
		A[i]=t-sumD[h];
	}
	sort(A+1,A+m+1);
	for(int i=1;i<=m;i++)
		sumA[i]=sumA[i-1]+A[i];
	memset(f,0x3f,sizeof(f));
	f[0][0]=0;
	for(int i=1;i<=p;i++){
		q[l=r=1]=0;
		for(int j=1;j<=m;j++){
			ll nowK=A[j];
			while(l<r&&f[i-1][q[l+1]]+sumA[q[l+1]]-f[i-1][q[l]]-sumA[q[l]]<nowK*(q[l+1]-q[l]))l++;
			f[i][j]=f[i-1][q[l]]+sumA[q[l]]-q[l]*A[j]+j*A[j]-sumA[j];
			while(l<r&&(f[i-1][q[r]]+sumA[q[r]]-f[i-1][q[r-1]]-sumA[q[r-1]])*(j-q[r])
						>(f[i-1][j]+sumA[j]-f[i-1][q[r]]-sumA[q[r]])*(q[r]-q[r-1]))r--;
			q[++r]=j;
		}
	}
	printf("%lld\n",f[p][m]);
	return 0;
}
```