## 思路讲解：

先将 $p_i$ 替换成 $k_i - p_i$，则原题是使现在的变为全零。 接下来就可以用贪心了。

## 代码部分：

```cpp
#include <bits/stdc++.h>
using namespace std;

const int N = 1010;
int a[N], b[N], c[N];

int main() {
    ios::sync_with_stdio(false), cin.tie(0);
    int n;
    cin >> n;
    for (int i = 1; i <= n; i++) {
        cin >> a[i];
    }
    for (int i = 1; i <= n; i++) {
        cin >> b[i];
        c[i] = b[i] - a[i];
    }
    int ans = 0;
    for (int i = 1; i <= n; i++) {
        if (c[i] >= 0 && c[i - 1] >= 0) {
            ans += max(0, c[i] - c[i - 1]);
        } else if (c[i] <= 0 && c[i - 1] <= 0) {
            ans += max(0, c[i - 1] - c[i]);
        } else if (c[i] >= 0 && c[i - 1] <= 0) {
            ans += c[i];
        } else {
            ans += -c[i];
        }
    }
    cout << ans << "\n";
    return 0;
}
```