稍微扰动一下就好了。

$$\sum_{i=1}^n i^k a^i=\sum_{i=1}^{n-1}i^k a^i +n^k a^n=\sum_{i=1}^{n-1}(i+1)^k a^{i+1}+a$$

$$\therefore \sum_{i=1}^{n-1}[(i+1)^ka^{i+1}-i^k a^i]=n^ka^n-a$$

对$(i+1)^k$二项式展开

$$\sum_{i=1}^{n-1}[a^{i+1}\sum_{j=0}^k\binom{k}{j}i^j -i^k a^i]=n^ka^n-a$$

$$\sum_{i=1}^{n-1}[a^{i+1}\sum_{j=0}^{k-1}\binom{k}{j}i^j + i^ka^{i+1} -i^k a^i]=n^ka^n-a$$

$$\sum_{i=1}^{n-1}a^{i+1}\sum_{j=0}^{k-1}\binom{k}{j}i^j + (a-1)\sum_{i=1}^{n-1}i^k a^i=n^ka^n-a$$

$$\sum_{j=0}^{k-1}\binom{k}{j}\sum_{i=1}^{n-1}a^{i+1}i^j + (a-1)\sum_{i=1}^{n-1}i^k a^i=n^ka^n-a$$

$$a\sum_{j=0}^{k-1}\binom{k}{j}\sum_{i=1}^{n-1}i^j a^i + (a-1)\sum_{i=1}^{n-1}i^k a^i=n^ka^n-a$$

设$$F(k)=\sum_{i=0}^{n-1} i^k a^i$$

$$a\sum_{j=0}^{k-1}\binom{k}{j}F(j) + (a-1)F(k)=n^ka^n-a$$

$$(a-1)F(k)=-a\sum_{j=0}^{k-1}\binom{k}{j}F(j) +n^ka^n-a$$

$$F(k)=\dfrac{-a\sum_{j=0}^{k-1}\binom{k}{j}F(j) +n^ka^n-a}{a-1}$$

我们可以很容易算出$F(0)$的值，然后预处理组合数，就可以在$O(k^2)$时间内递推出$F(k)$。

最后的答案为$F(k)+n^k a^n$。

---

那$a=1$呢？

此时有

$$\sum_{j=0}^{k-1}\binom{k}{j}F(j)=n^k-1$$

$$F(k-1)\times\binom{k}{k-1}+ \sum_{j=0}^{k-2}\binom{k}{j}F(j)=n^k-1$$

$$F(k-1)\times \binom{k}{k-1}=n^k-1-\sum_{j=0}^{k-2}\binom{k}{j}F(j)$$

$$F(k-1)=\dfrac{n^k-1-\sum_{j=0}^{k-2}\binom{k}{j}F(j)}{\binom{k}{k-1}}$$

即

$$F(k)=\dfrac{n^{k+1}-\sum_{j=0}^{k-1}\binom{k+1}{j}F(j)}{\binom{k+1}{k}}$$