此题就是求 $\sum\limits_{i=n}^{m}{fib}_i$。

$fib_i=fib_{i-1}+fib_{i-2}$

$fib_{i-1}=fib_{i-2}+fib_{i-3}$

$fib_i=fib_{i-2}+fib_{i-2}+fib_{i-3}$

$fib_{i-2}=fib_{i-3}+fib_{i-4}$

$fib_i=fib_{i-2}+fib_{i-3}+fib_{i-3}+fib_{i-4}$

由此推出 $fib_n-fib_1=\sum\limits_{i=1}^{n-2}fib_i$。

所以只需要求出 $fib_{m+2}-fib_{n+1}$ 即可。

$fib_{2n+1}={fib_{n+1}}^2+{fib_{n}}^{2}$

$fib_{2n}={fib_{n+1}}^2-{fib_{n-1}}^{2}$

用 map 记忆化搜索即可。

Code:

```cpp
#include<iostream>
#include<map>
using namespace std;
typedef long long ll;
const ll MOD=1e9+7;
map<ll,ll> mp;
map<ll,ll>::iterator it;
ll dg(ll n){
	if(n<=2){
		return 1ll;
	}
	it=mp.find(n);
	if(it!=mp.end()){
		return mp[n];
	}
	if(!(n&1)){
		return mp[n]=((dg(n/2-1)*2+dg(n>>1))%MOD*dg(n>>1))%MOD;
	}
	return mp[n]=(dg(n/2+1)*dg(n/2+1)%MOD+MOD+dg(n>>1)*dg(n>>1)%MOD)%MOD;
}
int main(){
	long long n,m,t;
	cin>>t; 
	while(t--){
		cin>>n>>m;
		cout<<(dg(m+2)-dg(n+1)+MOD)%MOD<<endl;
	}
	return 0;
}
```
