初始矩阵我们记作fst，递推矩阵记作trans ↓

**1 1 1**    **1 1 0**

**0 0 0**    **0 0 1**

**0 0 0**    **1 0 0**

那么fst+1=fst\*trans,fst+2=(fst+1)\*trans……

易得ans=fst\*(trans^(n-3))

注意乘积爆int需要强转long long。

另外n<=3的情况需要特判，这道题就做完了。


```cpp
#include<cstdio>
#include<cstring>
#include<algorithm>
#define mod 1000000007 
using namespace std;
int n; 
struct Mat 
{
    int x,y;
    int arr[5][5];
    Mat(){}
    Mat(const int _x,const int _y)
    {
        x=_x,y=_y; 
        memset(arr,0,sizeof(arr)); 
    }
    void unit()
    {
        for(int i=1;i<=x;++i) arr[i][i]=1; 
    }
    Mat operator*(Mat b)
    {
        Mat a=*this,c(a.x,b.y);
        for(int i=1;i<=c.x;++i)
            for(int j=1;j<=c.y;++j)
                for(int k=1;k<=a.y;++k)
                    (c.arr[i][j]+=(long long)a.arr[i][k]*b.arr[k][j]%mod)%=mod;
        return c; 
    }
    Mat operator^(const int B)
    {
        int b=B; 
        Mat ret(3,3),X=*this;
        ret.unit();
        while(b){
            if(b&1) ret=ret*X;
            X=X*X; 
            b>>=1; 
        }
        return ret; 
    }
};
int main()
{
    int T;
    scanf("%d",&T);
    while(T--){
        scanf("%d",&n);
        if(n<=3){
            printf("%d\n",1);
            continue; 
        }
         Mat trans(3,3),fst(3,3);
        trans.arr[1][1]=trans.arr[1][2]=trans.arr[2][3]=trans.arr[3][1]=fst.arr[1][1]=fst.arr[1][2]=fst.arr[1][3]=1;
        Mat ans=fst*(trans^(n-3)); 
        printf("%d\n",ans.arr[1][1]); 
    }
    return 0; 
} 
```