相信这道题很多人写的代码很长，实际上运用同余定理很轻松。

举例说明：123%11=（100%11+20%11+3%11）%11=（（1%11\*10+2）%11\*10+3）%11

```cpp
[color=red]
#include <cstdio>
#include <iostream>
#include <cstring>
using namespace std;
string m;
int a[1010]={0};
int main()
{
    int n;
    cin>>n;
    cin>>m;
    for(int i=0;i<m.size();i++)
        a[i]=m[i]-'0';
    long long ans=0;
    for(int i=0;i<m.size();i++)
        ans=(ans*10+a[i])%n;//公式运用在这里
    if(ans==0) cout<<n<<endl;
    else cout<<ans<<endl;
    return 0;
}
[/color][codec ]
```