前置芝士：快速幂

$\sum\limits_{i=a}^{b}F(i,k)$ 即为 $\sum\limits_{i=1}^{b}F(i,k)-\sum\limits_{i=1}^{a-1}F(i,k)$ 。

所以我们只需求出 $\sum\limits_{i=1}^{x}F(i,k)$ 即可 。

$\sum\limits_{i=1}^{x}F(i,k)$

$=\sum\limits_{i=1}^{x}\sum\limits_{j|i}j^k$

枚举 $j$ ：

$=\sum\limits_{i=1}^{x}\left\lfloor\dfrac{x}{i}\right\rfloor\times i^k$

快速幂推过去即可 。

Code：

```cpp
#include<iostream>
using namespace std;
typedef long long ll;
const ll mod=1e9+7;
ll pre(ll x,ll s,ll k){
	ll ans=1;
	while(s){
		if(s&1){
			ans=(ans*x)%k;
		}
		x=(x*x)%k;
		s>>=1;
	}
	return ans;
}
ll sum(ll n,ll k){
	ll ans=0;
	for(ll i=1;i<=n;i++){
		ans+=pre(i,k,mod)*(n/i);
		ans%=mod;
	}
	return ans;
}
int main(){
	int t;
	cin>>t;
	ll a,b,k;
	while(t--){
		cin>>a>>b>>k;
		cout<<(sum(b,k)-sum(a-1,k)+mod)%mod<<endl;
	}
	return 0;
} 
```
