假设 $n \le m$

$$ \begin{aligned} &\prod_{i=1}^{n}\prod_{j=1}^{m}f(\gcd(i,j)) \\ =&\prod_{d=1}^{n}f(d)^{\sum_{i=1}^{n}\sum_{j=1}^{m}[\gcd(i,j)=d]} \\ =&\prod_{d=1}^{n}f(d)^{\sum_{i=1}^{\lfloor \frac{n}{d} \rfloor}\sum_{j=1}^{\lfloor \frac{m}{d} \rfloor}[\gcd(i,j)=1]} \\ =&\prod_{d=1}^{n}f(d)^{\sum_{i=1}^{\lfloor \frac{n}{d} \rfloor}\sum_{j=1}^{\lfloor \frac{m}{d} \rfloor}\sum_{t \mid \gcd(i,j)}\mu(t)} \\ =&\prod_{d=1}^{n}f(d)^{\sum_{t = 1}^{\lfloor \frac{n}{d} \rfloor}\mu(t)\sum_{i=1}^{\lfloor \frac{n}{d} \rfloor}\sum_{j=1}^{\lfloor \frac{m}{d} \rfloor}[t \mid \gcd(i,j)]} \\ =&\prod_{d=1}^{n}f(d)^{\sum_{t = 1}^{\lfloor \frac{n}{d} \rfloor}\mu(t)\sum_{i=1}^{\lfloor \frac{n}{d} \rfloor}\sum_{j=1}^{\lfloor \frac{m}{d} \rfloor}[t \mid i][t \mid j]} \\ =&\prod_{d=1}^{n}f(d)^{\sum_{t = 1}^{\lfloor \frac{n}{d} \rfloor}\mu(t)\sum_{i=1}^{\lfloor \frac{n}{d} \rfloor}[t \mid i]\sum_{j=1}^{\lfloor \frac{m}{d} \rfloor}[t \mid j]} \\ =&\prod_{d=1}^{n}f(d)^{\sum_{t = 1}^{\lfloor \frac{n}{d} \rfloor}\mu(t)\lfloor \frac{n}{dt} \rfloor \lfloor \frac{m}{dt} \rfloor} \\ =&\prod_{T=1}^{n}\prod_{d \mid T}f(d)^{\mu(\frac{T}{d})\lfloor \frac{n}{T} \rfloor \lfloor \frac{m}{T} \rfloor} \\ =&\prod_{T=1}^{n} \left( \prod_{d \mid T}f(d)^{\mu ( \frac{T}{d} ) } \right) ^ { \lfloor \frac{n}{T} \rfloor \lfloor \frac{m}{T} \rfloor} \\ =&\prod_{T=1}^{n} g(T) ^ { \lfloor \frac{n}{T} \rfloor \lfloor \frac{m}{T} \rfloor} \\ \end{aligned} $$

然后就可以对 $\lfloor \frac{n}{T} \rfloor \lfloor \frac{m}{T} \rfloor$ 进行数论分块了，然后考虑如何求 $g(T)$

首先有：

$$ g(T)=\sum_{d \mid T} f(d)^{\mu(\frac{T}{d})} $$

显然 $f,\mu$ 都可以预处理出来，之后只需要枚举 $i$，再枚举 $j$，用 $f(i) ^ {\mu(j)}$ 累加到 $g(i \times j)$ 上就行了