喜闻乐见的推柿子。

$\sum_i \sum_j (i+j)^k f(\gcd(i,j))\gcd(i,j)$

根据 $f$ 的定义我们发现 $f = \mu^2$。

然后随便推。

$\sum_i \sum_j (i+j)^K \mu^2(\gcd(i,j))\gcd(i,j)$

$\sum_d \mu^2(d) d\sum_i \sum_j (id+jd)^K [\gcd =1]$

$\sum_d \mu^2(d) d^{K+1}\sum_i \sum_j (i+j)^K[\gcd=1]$

$\sum_d \mu^2(d) d^{K+1}\sum_i \sum_j (i+j)^K\sum_{k|\gcd(i,j)}\mu_k$

$\sum_d \mu^2(d) d^{K+1} \sum_k \mu(k) k^{K}\sum_i \sum_j (i+j)^k$

$F(n) = \sum_i \sum_j (i+j)^k$。

$T=dk$。

$\sum_{T} T^K\times  F(\frac{n}{T})\sum_{d|T} \mu^2(d)d \mu(\frac{T}{d})$。

$f(n) = \sum_{i}^{n} i^k$。
$g(n) = \sum_{i}^{n} f(i)$。

显然 $F(n) = g(2n) - 2g(n)$。

$\sum_{T} T^K\times  (g(\frac{2n}{T}) - 2g(\frac{n}{T}))\sum_{d|T} \mu^2(d)d \mu(\frac{T}{d})$。

所以做完了？