### 一种不用分块的做法
先把要求的东西表示成数学式子 ：
$$\sum\limits_{i=x}^{y}\sum\limits_{d\mid i}d$$
令 $f(n)=\sum\limits_{i=1}^{n}\sum\limits_{d\mid i}d$ ，转为枚举 d ，可得 ：
$$f(n)=\sum\limits_{d=1}^{n}d\left\lfloor\dfrac{n}{d}\right\rfloor$$
到这里可以分块算 。
$$=\sum\limits_{i=1}^{n}\sum\limits_{j=1}^{n}i\left[i\times j\le n\right]$$
$$=\sum\limits_{i=1}^{\left\lfloor\sqrt{n}\right\rfloor}\sum\limits_{j=1}^{\left\lfloor\frac{n}{i}\right\rfloor}i+\sum\limits_{j=1}^{\left\lfloor\sqrt{n}\right\rfloor}\sum\limits_{i=1}^{\left\lfloor\frac{n}{j}\right\rfloor}i-\sum\limits_{i=1}^{\left\lfloor\sqrt{n}\right\rfloor}\sum\limits_{j=1}^{\left\lfloor\sqrt{n}\right\rfloor}i$$
$$=\sum\limits_{i=1}^{\left\lfloor\sqrt{n}\right\rfloor}i\left\lfloor\dfrac{n}{i}\right\rfloor+\sum\limits_{j=1}^{\left\lfloor\sqrt{n}\right\rfloor}\left\lfloor\frac{n}{j}\right\rfloor\left(\left\lfloor\frac{n}{j}\right\rfloor+1\right)-\left\lfloor\sqrt{n}\right\rfloor\sum\limits_{i=1}^{\left\lfloor\sqrt{n}\right\rfloor}i$$
$$=\dfrac{\sum\limits_{i=1}^{\left\lfloor\sqrt{n}\right\rfloor}\left\lfloor\dfrac{n}{i}\right\rfloor\left(\left\lfloor\dfrac{n}{i}\right\rfloor+2i+1\right)-\left\lfloor\sqrt{n}\right\rfloor^{2}\left(\left\lfloor\sqrt{n}\right\rfloor+1\right)}{2}$$
然后就可以直接算了。
```cpp
#include <cmath>
#include <iostream>
using namespace std;
#define ll long long
ll sum(int n) {
	ll ans=0;
	int sqrn=sqrt(n);
	for(int i=1; i<=sqrn; ++i) ans+=(n/i)*(ll)(n/i+2*i+1);
	return (ans-sqrn*sqrn*(ll)(sqrn+1))>>1;
}
int main() {
	int x,y;
	cin>>x>>y;
	cout<<sum(y)-sum(x-1);
	return 0;
}
```
