这是一道很简单的题

考虑当 $n>0$ 时，答案一定会是 $l=-(n-1)=-n+1$，$r=n$ 。

此时，原式 $=\displaystyle\sum_{i=1}^n-\displaystyle\sum_{i=1}^{n-1}$

易知答案为 $n$。

当 $n=0$ 时，直接输出```-1 1```就行了

当 $n<0$ 时，答案为 $l=n$ ，$r=-(n+1)$

此时，原式 $=\displaystyle\sum_{i=1}^{-n-1}-\displaystyle\sum_{i=1}^{-n}$

易知答案为 $n$

代码：
```cpp
#include<bits/stdc++.h>
#define int long long
using namespace std;
int t;
signed main()
{
    cin>>t;
    for(int i=1;i<=t;i++)
    {
        int n;
        cin>>n;
        if(n>0)
            cout<<-(n-1)<<' '<<n<<endl;
        if(n==0)
            cout<<-1<<' '<<1<<endl;
        if(n<0)
        {
            cout<<n<<' '<<-(n+1)<<endl;
        }
    }
    return 0;
}
```